heap/tree_down.v
@@ -1,0 +1,606 @@
+Require Import FloydSeq.proofauto.
+(* Require Import cprogs.heap.program. *)
+Require Import Notations Logic Datatypes.
+From Coq Require Import String List ZArith. 
+From compcert Require Import Coqlib Integers Floats AST Ctypes Cop Clight Clightdefs.
+Require Import Coq.Logic.Classical_Pred_Type.
+Require Import Classical_Prop.
+
+Require Import Coq.micromega.Psatz.
+Local Open Scope string.
+Local Open Scope nat_scope.
+Local Open Scope Z_scope.
+Local Open Scope list_scope.
+Require Import cprogs.heap.list_relation.
+Require Import cprogs.heap.definitions.
+Require Import cprogs.heap.tree_list.
+
+Require Import SetsClass.SetsClass.
+Local Open Scope sets.
+Import SetsNotation.
+
+Definition MaxHeap_tree_down(ts: tree_state): Prop :=
+  MaxHeap_partial_tree_v (fst ts) (get_tree_val (snd ts)) /\ MaxHeap_no_rt (snd ts) /\
+  (exists v ls rs, snd ts = Node v ls rs /\
+  (ls = Leaf \/ MaxHeap_partial_tree_v (fst ts) (get_tree_val ls)) /\
+  (rs = Leaf \/ MaxHeap_partial_tree_v (fst ts) (get_tree_val rs))).
+
+Lemma left_son_check_equal: forall l n v ls rs,
+  list_nth_on_tree l n (Node v ls rs) ->
+  left_son_check_list (l, n) <-> left_son_check_tree v ls rs.
+Proof.
+  intros.
+  inversion H; [discriminate | ].
+  inversion H0; subst.
+  split; intros.
+  + unfold left_son_check_list in H2.
+    unfold left_son in H2; simpl in H2.
+    destruct H2 as [? ?].
+    unfold legal_list_state in H2; simpl in H2.
+    inversion H3; [lia | subst].
+    unfold left_son_check_tree; split.
+    - unfold not; intros.
+      discriminate.
+    - unfold get_tree_val.
+      unfold get_list_val in H5; simpl in H5.
+      replace (n * 2) with (2 * n) by lia.
+      lia.
+  + unfold left_son_check_tree in H2; destruct H2.
+    inversion H3; [tauto | subst].
+    unfold left_son_check_list; unfold left_son; simpl.
+    split.
+    - unfold legal_list_state; simpl; lia.
+    - unfold get_list_val; simpl.
+      unfold get_tree_val in H5.
+      replace (n * 2) with (2 * n) in H5 by lia.
+      lia.
+Qed.
+
+Lemma right_son_check_equal: forall l n v ls rs,
+  list_nth_on_tree l n (Node v ls rs) ->
+  right_son_check_list (l, n) <-> right_son_check_tree v ls rs.
+Proof.
+  intros.
+  inversion H; [discriminate | ].
+  inversion H0; subst.
+  split; intros.
+  + unfold right_son_check_list in H2.
+    unfold right_son in H2; simpl in H2.
+    destruct H2 as [? ?].
+    unfold legal_list_state in H2; simpl in H2.
+    inversion H4; [lia | subst].
+    unfold right_son_check_tree; split.
+    - unfold not; intros.
+      discriminate.
+    - unfold get_tree_val.
+      unfold get_list_val in H5; simpl in H5.
+      replace (n * 2) with (2 * n) by lia.
+      lia.
+  + unfold right_son_check_tree in H2; destruct H2.
+    inversion H4; [tauto | subst].
+    unfold right_son_check_list; unfold right_son; simpl.
+    split.
+    - unfold legal_list_state; simpl; lia.
+    - unfold get_list_val; simpl.
+      unfold get_tree_val in H5.
+      replace (n * 2) with (2 * n) in H5 by lia.
+      lia.
+Qed.
+
+Lemma converse_neg: forall (P Q: Prop),
+  (P -> Q) -> (~ Q -> ~ P).
+Proof.
+  intros.
+  unfold not; intros.
+  apply H0; apply H; assumption.
+Qed.
+
+Lemma swap_down_left_hold: forall l n l' n' pt v ls rs v0 ls0 rs0,
+  list_on_tree_state (l, n) (pt, Node v ls rs) ->
+  left_son_swap (l, n) (l', n') ->
+  ls = Node v0 ls0 rs0 ->
+  list_on_tree_state (l', n') ((false, v0, rs) :: pt, Node v ls0 rs0).
+Proof.
+  intros.
+  unfold list_on_tree_state in H.
+  unfold list_on_tree_state_fix in H.
+  simpl in H; destruct H as [? ?].
+  subst.
+  unfold left_son_swap in H0; simpl in H0.
+  destruct H0; subst.
+  inversion H; [discriminate | ].
+  inversion H1; subst v1 ls rs1.
+  inversion H5; [discriminate | ].
+  inversion H4; subst v1 ls rs1.
+  pose proof list_swap_rela_rewrite l l' n (2 * n) ltac:(lia) ltac:(lia) H0.
+  subst l'.
+  assert (Zlength (list_swap l n (2 * n)) = Zlength l). {
+    rewrite list_swap_Zlength by lia; lia.
+  }
+  assert (Zlength (upd_Znth (2 * n) l (Znth n l)) = Zlength l). {
+    rewrite upd_Znth_Zlength; lia.
+  }
+  assert (Zlength (upd_Znth (n * 2) l (Znth n l)) = Zlength l). {
+    rewrite upd_Znth_Zlength; lia.
+  }
+  unfold list_on_tree_state.
+  unfold list_on_tree_state_fix.
+  simpl; split.
+  + eapply list_nth_on_tree_Node; eauto.
+    - lia.
+    - unfold list_swap.
+      rewrite upd_Znth_diff by lia.
+      rewrite upd_Znth_same by lia; reflexivity.
+    - unfold list_swap.
+      apply list_nth_on_tree_upd; [ | lia | ].
+      * apply list_nth_on_tree_upd; [ | lia | ].
+        ++ replace (2 * n) with (n * 2) by lia; assumption.
+        ++ apply less_is_not_child_index; lia.
+      * apply less_is_not_child_index; lia.
+    - unfold list_swap.
+      apply list_nth_on_tree_upd; [ | lia | ].
+      * apply list_nth_on_tree_upd; [ | lia | ].
+        ++ replace (2 * n) with (n * 2) by lia; assumption.
+        ++ apply less_is_not_child_index; lia.
+      * apply less_is_not_child_index; lia.
+  + eapply cons_partial_tree; eauto; simpl.
+    - lia.
+    - replace (2 * n) with (n * 2) by lia; rewrite Z.div_mul by lia; lia.
+    - replace (2 * n) with (n * 2) by lia; rewrite Z.div_mul by lia.
+      unfold list_swap.
+      rewrite upd_Znth_same by lia; reflexivity.
+    - unfold list_swap.
+      apply list_nth_on_tree_upd; [ | lia | ].
+      * apply list_nth_on_tree_upd; [ | lia | ].
+        ++ replace (2 * n) with (n * 2) by lia; assumption.
+        ++ apply less_is_not_child_index; lia.
+      * apply less_is_not_child_index; lia.
+    - replace (2 * n) with (n * 2) by lia; rewrite Z.div_mul by lia.
+      apply list_on_partial_tree_upd; try lia.
+      * apply is_child_index_self; reflexivity.
+      * apply list_on_partial_tree_upd; try lia.
+        ++ apply is_child_index_gp_inv_left; [lia | ].
+           apply is_child_index_self; reflexivity.
+        ++ assumption.
+Qed.
+
+Lemma swap_down_right_hold: forall l n l' n' pt v ls rs v0 ls0 rs0,
+  list_on_tree_state (l, n) (pt, Node v ls rs) ->
+  right_son_swap (l, n) (l', n') ->
+  rs = Node v0 ls0 rs0 ->
+  list_on_tree_state (l', n') ((true, v0, ls) :: pt, Node v ls0 rs0).
+Proof.
+  intros.
+  unfold list_on_tree_state in H.
+  unfold list_on_tree_state_fix in H.
+  simpl in H; destruct H as [? ?].
+  subst.
+  unfold right_son_swap in H0; simpl in H0.
+  destruct H0; subst.
+  inversion H; [discriminate | ].
+  inversion H1; subst v1 ls1 rs.
+  inversion H6; [discriminate | ].
+  inversion H4; subst v1 ls1 rs.
+  pose proof list_swap_rela_rewrite l l' n (2 * n + 1) ltac:(lia) ltac:(lia) H0.
+  subst l'.
+  assert (Zlength (list_swap l n (2 * n + 1)) = Zlength l). {
+    rewrite list_swap_Zlength by lia; lia.
+  }
+  assert (Zlength (upd_Znth (2 * n + 1) l (Znth n l)) = Zlength l). {
+    rewrite upd_Znth_Zlength; lia.
+  }
+  assert (Zlength (upd_Znth (n * 2 + 1) l (Znth n l)) = Zlength l). {
+    rewrite upd_Znth_Zlength; lia.
+  }
+  unfold list_on_tree_state.
+  unfold list_on_tree_state_fix.
+  simpl; split.
+  + eapply list_nth_on_tree_Node; eauto.
+    - lia.
+    - unfold list_swap.
+      rewrite upd_Znth_diff by lia.
+      rewrite upd_Znth_same by lia; reflexivity.
+    - unfold list_swap.
+      apply list_nth_on_tree_upd; [ | lia | ].
+      * apply list_nth_on_tree_upd; [ | lia | ].
+        ++ replace (2 * n) with (n * 2) by lia; assumption.
+        ++ apply less_is_not_child_index; lia.
+      * apply less_is_not_child_index; lia.
+    - unfold list_swap.
+      apply list_nth_on_tree_upd; [ | lia | ].
+      * apply list_nth_on_tree_upd; [ | lia | ].
+        ++ replace (2 * n) with (n * 2) by lia; assumption.
+        ++ apply less_is_not_child_index; lia.
+      * apply less_is_not_child_index; lia.
+  + assert ((n * 2 + 1) / 2 = n). {
+      pose proof Z.div_lt_upper_bound (n * 2 + 1) 2 (n + 1) ltac:(lia) ltac:(lia).
+      pose proof Z.div_le_lower_bound (n * 2 + 1) 2 n ltac:(lia) ltac:(lia).
+      lia.
+    }
+    eapply cons_partial_tree; eauto; simpl.
+    - lia.
+    - replace (2 * n) with (n * 2) by lia; lia.
+    - replace (2 * n) with (n * 2) by lia. rewrite H15.
+      unfold list_swap.
+      rewrite upd_Znth_same by lia; reflexivity.
+    - unfold list_swap.
+      apply list_nth_on_tree_upd; [ | lia | ].
+      * apply list_nth_on_tree_upd; [ | lia | ].
+        ++ replace (2 * n + 1 + -1) with (n * 2) by lia; assumption.
+        ++ apply rchild_is_not_lchild with (pp := n); try lia.
+           apply is_child_index_self; lia.
+      * apply less_is_not_child_index; lia.
+    - replace (2 * n) with (n * 2) by lia; rewrite H15.
+      apply list_on_partial_tree_upd; try lia.
+      * apply is_child_index_self; reflexivity.
+      * apply list_on_partial_tree_upd; try lia.
+        ++ apply is_child_index_gp_inv_right; [lia | ].
+           apply is_child_index_self; reflexivity.
+        ++ assumption.
+Qed.
+
+Lemma MaxHeap_no_rt_impl_lchild: forall v ls rs,
+  MaxHeap_no_rt (Node v ls rs) -> MaxHeap ls.
+Proof.
+  intros.
+  unfold MaxHeap_no_rt in H.
+  destruct H as [v0 [ls0 [rs0 [? [? ?] ]] ] ].
+  inversion H; subst.
+  tauto.
+Qed.
+Lemma MaxHeap_no_rt_impl_rchild: forall v ls rs,
+  MaxHeap_no_rt (Node v ls rs) -> MaxHeap rs.
+Proof.
+  intros.
+  unfold MaxHeap_no_rt in H.
+  destruct H as [v0 [ls0 [rs0 [? [? ?] ]] ] ].
+  inversion H; subst.
+  tauto.
+Qed.
+Lemma MaxHeap_impl_MaxHeap_no_rt: forall v v0 ls rs, 
+  MaxHeap (Node v ls rs) -> MaxHeap_no_rt (Node v0 ls rs).
+Proof.
+  intros.
+  inversion H; [discriminate | ].
+  inversion H0; subst.
+  unfold MaxHeap_no_rt.
+  exists v0, ls0, rs0.
+  tauto.
+Qed.
+
+Lemma not_inequal_impl_equal: forall {A: Type} (a b: A),
+  ~ a <> b -> a = b.
+Proof.
+  intros.
+  destruct (classic (a = b)); [assumption | ].
+  unfold not in H at 1.
+  apply H in H0.
+  contradiction.
+Qed.
+
+Lemma MaxHeap_tree_down_hold_left: forall pt v ls rs v0 ls0 rs0,
+  MaxHeap_tree_down (pt, Node v ls rs) ->
+  ls = Node v0 ls0 rs0 ->
+  v0 >= v ->
+  (~ right_son_check_tree v ls rs \/ get_tree_val rs <= v0) ->
+  MaxHeap_tree_down ((false, v0, rs) :: pt, Node v ls0 rs0).
+Proof.
+  intros.
+  unfold MaxHeap_tree_down in H; simpl in H.
+  destruct H as [? [? [? [? [? [? [? ?] ] ] ] ] ] ].
+  inversion H4; subst x x0 x1 ls.
+  unfold MaxHeap_tree_down; simpl.
+  unfold get_tree_val in H5; simpl in H5.
+  destruct H5; [discriminate | ].
+  unfold right_son_check_tree in H2.
+  split; [ | split].
+  - eapply MaxHeap_partial_tree_v_app; eauto.
+    * eapply MaxHeap_no_rt_impl_rchild; eauto.
+    * destruct rs; [tauto | right].
+      unfold get_tree_val.
+      destruct H2.
+      ++ apply not_and_or in H2.
+         destruct H2; [apply not_inequal_impl_equal in H2; discriminate | ].
+         unfold get_tree_val in H2; lia.
+      ++ unfold get_tree_val in H2; lia. 
+    * lia.
+  - pose proof MaxHeap_no_rt_impl_lchild _ _ _ H3.
+    eapply MaxHeap_impl_MaxHeap_no_rt; eauto.
+  - exists v, ls0, rs0.
+    split; [reflexivity | split].
+    * destruct ls0; [tauto | right].
+      unfold get_tree_val.
+      eapply MaxHeap_partial_tree_v_app; eauto.
+      ++ eapply MaxHeap_no_rt_impl_rchild; eauto.
+      ++ destruct H2; [ | tauto].
+         apply not_and_or in H2.
+         destruct H2; [left; apply not_inequal_impl_equal; tauto | right; lia].
+      ++ pose proof MaxHeap_no_rt_impl_lchild _ _ _ H3.
+         inversion H5; [discriminate | ].
+         inversion H7; subst v2 ls rs1.
+         destruct H10; [discriminate | ].
+         unfold get_tree_val in H10; lia.
+    * destruct rs0; [tauto | right].
+      unfold get_tree_val.
+      eapply MaxHeap_partial_tree_v_app; eauto.
+      ++ eapply MaxHeap_no_rt_impl_rchild; eauto.
+      ++ destruct H2; [ | tauto].
+         apply not_and_or in H2.
+         destruct H2; [left; apply not_inequal_impl_equal; tauto | right; lia].
+      ++ pose proof MaxHeap_no_rt_impl_lchild _ _ _ H3.
+         inversion H5; [discriminate | ].
+         inversion H7. subst v2 ls rs0.
+         destruct H11; [discriminate | ].
+         unfold get_tree_val in H11; lia. 
+Qed.
+
+Lemma MaxHeap_tree_down_hold_right: forall pt v ls rs v0 ls0 rs0,
+  MaxHeap_tree_down (pt, Node v ls rs) ->
+  rs = Node v0 ls0 rs0 ->
+  v0 >= v ->
+  (~ left_son_check_tree v ls rs \/ get_tree_val ls <= v0) ->
+  MaxHeap_tree_down ((true, v0, ls) :: pt, Node v ls0 rs0).
+Proof.
+  intros.
+  unfold MaxHeap_tree_down in H; simpl in H.
+  destruct H as [? [? [? [? [? [? [? ?] ] ] ] ] ] ].
+  inversion H4. subst x x0 x1 rs.
+  unfold MaxHeap_tree_down; simpl.
+  unfold get_tree_val in H6; simpl in H6.
+  destruct H6; [discriminate | ].
+  unfold left_son_check_tree in H2.
+  split; [ | split].
+  - eapply MaxHeap_partial_tree_v_app; eauto.
+    * eapply MaxHeap_no_rt_impl_lchild; eauto.
+    * destruct ls; [tauto | right].
+      unfold get_tree_val.
+      destruct H2.
+      ++ apply not_and_or in H2.
+         destruct H2; [apply not_inequal_impl_equal in H2; discriminate | ].
+         unfold get_tree_val in H2; lia.
+      ++ unfold get_tree_val in H2; lia. 
+    * lia.
+  - pose proof MaxHeap_no_rt_impl_rchild _ _ _ H3.
+    eapply MaxHeap_impl_MaxHeap_no_rt; eauto.
+  - exists v, ls0, rs0.
+    split; [reflexivity | split].
+    * destruct ls0; [tauto | right].
+      unfold get_tree_val.
+      eapply MaxHeap_partial_tree_v_app; eauto.
+      ++ eapply MaxHeap_no_rt_impl_lchild; eauto.
+      ++ destruct H2; [ | tauto].
+         apply not_and_or in H2.
+         destruct H2; [left; apply not_inequal_impl_equal; tauto | right; lia].
+      ++ pose proof MaxHeap_no_rt_impl_rchild _ _ _ H3.
+         inversion H6; [discriminate | ].
+         inversion H7. subst v2 ls0 rs.
+         destruct H10; [discriminate | ].
+         unfold get_tree_val in H10; lia.
+    * destruct rs0; [tauto | right].
+      unfold get_tree_val.
+      eapply MaxHeap_partial_tree_v_app; eauto.
+      ++ eapply MaxHeap_no_rt_impl_lchild; eauto.
+      ++ destruct H2; [ | tauto].
+         apply not_and_or in H2.
+         destruct H2; [left; apply not_inequal_impl_equal; tauto | right; lia].
+      ++ pose proof MaxHeap_no_rt_impl_rchild _ _ _ H3.
+         inversion H6; [discriminate | ].
+         inversion H7. subst v2 ls1 rs.
+         destruct H11; [discriminate | ].
+         unfold get_tree_val in H11; lia. 
+Qed.
+
+Lemma Down_tree_list_succeed: forall (l l': list_state) (t: tree_state),
+  list_on_tree_state l t -> list_down_succeed l l' -> MaxHeap_tree_down t ->
+  exists t', tree_down_succeed t t' /\ list_on_tree_state l' t' /\ MaxHeap_tree_down t'.
+Proof.
+  intros.
+  unfold list_down_succeed in H0.
+  remember H1 as H1'; clear HeqH1'.
+  unfold MaxHeap_tree_down in H1.
+  destruct H1 as [? [? ?] ].
+  destruct H3 as [v [ls [rs ?]]].
+  destruct t as [pt tr].
+  destruct l as [l n].
+  destruct l' as [l' n'].
+  simpl in H3; simpl in H2; simpl in H1.
+  destruct H3 as [? [? ?] ]; subst.
+  remember H as H'; clear HeqH'.
+  unfold list_on_tree_state in H.
+  unfold list_on_tree_state_fix in H.
+  simpl in H; destruct H as [? ?].
+  inversion H; [discriminate | ].
+  inversion H6; subst v0 ls0 rs0.
+  destruct H0; [ | destruct H0].
+  {
+    destruct H0 as [? [? ?] ].
+    remember H0 as H0'; clear HeqH0'.
+    unfold left_son_check_list in H0.
+    unfold left_son in H0; simpl in H0.
+    destruct H0.
+    remember H8 as H8'; clear HeqH8'.
+    apply not_and_or in H8.
+    unfold legal_list_state in H0; simpl in H0.
+    inversion H9; [lia | ].
+    rewrite H14 in H4.
+    destruct H4; [discriminate | unfold get_tree_val in H4].
+    exists ((false, v0, rs) :: pt, Node v ls0 rs0).
+    split; [| split].
+    + unfold tree_down_succeed.
+      exists (false, v0, rs); simpl.
+      split; [reflexivity | ].
+      exists v, ls, rs.
+      split; [rewrite <- H12; reflexivity | ].
+      left; split; [| split].
+      - eapply left_son_check_equal; eauto.
+      - rewrite <- right_son_check_equal; eauto.
+      - unfold swap_down_left.
+        exists v0, ls0, rs0; tauto.
+    + eapply swap_down_left_hold; eauto.
+    + eapply MaxHeap_tree_down_hold_left; eauto.
+      - unfold get_list_val in H13; simpl in H13.
+        replace (2 * n) with (n * 2) in H13 by lia; lia.
+      - rewrite <- right_son_check_equal; eauto.
+  } {
+    destruct H0 as [? [? ?] ].
+    remember H0 as H0'; clear HeqH0'.
+    remember H8 as H8'; clear HeqH8'.
+    unfold left_son_check_list in H0.
+    unfold left_son in H0; simpl in H0.
+    unfold right_son_check_list in H8.
+    unfold right_son in H8; simpl in H8.
+    unfold left_son in H11; unfold right_son in H11; simpl in H11.
+    destruct H0, H8.
+    unfold legal_list_state in H8; simpl in H8.
+    inversion H9; [lia | ].
+    rewrite H15 in H4.
+    destruct H4; [discriminate | unfold get_tree_val in H4].
+    inversion H10; [lia | ].
+    rewrite H20 in H5.
+    destruct H5; [discriminate | unfold get_tree_val in H5].
+    destruct H11; destruct H11 as [H11a H11b].
+    + exists ((false, v0, rs) :: pt, Node v ls0 rs0).
+      assert (get_tree_val rs <= get_tree_val ls). {
+        rewrite H15, H20; unfold get_tree_val.
+        unfold get_list_val in H11a; simpl in H11a.
+        replace (2 * n) with (n * 2) in H11a by lia.
+        lia.
+      }
+      split; [| split].
+      - unfold tree_down_succeed.
+        exists (false, v0, rs); simpl.
+        split; [reflexivity | ].
+        exists v, ls, rs.
+        split; [rewrite <- H12; reflexivity | ].
+        right. right.
+        split; [| split].
+        * eapply left_son_check_equal; eauto.
+        * eapply right_son_check_equal; eauto.
+        * right. split; [lia | ].
+          unfold swap_down_left.
+          exists v0, ls0, rs0; tauto.
+      - eapply swap_down_left_hold; eauto.
+      - eapply MaxHeap_tree_down_hold_left; eauto.
+        * unfold get_list_val in H14; simpl in H14.
+          replace (2 * n) with (n * 2) in H14 by lia.
+          unfold get_list_val in H11a; simpl in H11a.
+          replace (2 * n) with (n * 2) in H11a by lia.
+          lia.
+        * rewrite H15 in H11.
+          unfold get_tree_val in H11 at 2.
+          lia.
+    + exists ((true, v1, ls) :: pt, Node v ls1 rs1).
+      assert (get_tree_val rs > get_tree_val ls). {
+        rewrite H15, H20; unfold get_tree_val.
+        unfold get_list_val in H11a; simpl in H11a.
+        replace (2 * n) with (n * 2) in H11a by lia.
+        lia.
+      }
+      split; [| split].
+      - unfold tree_down_succeed.
+        exists (true, v1, ls); simpl.
+        split; [reflexivity | ].
+        exists v, ls, rs.
+        split; [rewrite <- H12; reflexivity | ].
+        right. right.
+        split; [| split].
+        * eapply left_son_check_equal; eauto.
+        * eapply right_son_check_equal; eauto.
+        * left. split; [lia | ].
+          unfold swap_down_right.
+          exists v1, ls1, rs1; tauto.
+      - eapply swap_down_right_hold; eauto.
+      - eapply MaxHeap_tree_down_hold_right; eauto.
+        * unfold get_list_val in H14; simpl in H14.
+          replace (2 * n) with (n * 2) in H14 by lia.
+          unfold get_list_val in H11a; simpl in H11a.
+          replace (2 * n) with (n * 2) in H11a by lia.
+          lia.
+        * rewrite H20 in H11.
+          unfold get_tree_val in H11 at 1.
+          lia.
+  } {
+    destruct H0 as [? [? ?] ].
+    remember H0 as H0'; clear HeqH0'.
+    remember H8 as H8'; clear HeqH8'.
+    unfold right_son_check_list in H8.
+    unfold right_son in H8; simpl in H8.
+    destruct H8.
+    apply not_and_or in H0.
+    unfold legal_list_state in H8; simpl in H8.
+    inversion H10; [lia | ].
+    rewrite H14 in H5.
+    destruct H5; [discriminate | unfold get_tree_val in H5].
+    exists ((true, v0, ls) :: pt, Node v ls0 rs0).
+    split; [| split].
+    + unfold tree_down_succeed.
+      exists (true, v0, ls); simpl.
+      split; [reflexivity | ].
+      exists v, ls, rs.
+      split; [rewrite <- H12; reflexivity | ].
+      right; left; split; [| split].
+      - rewrite <- left_son_check_equal; eauto.
+      - eapply right_son_check_equal; eauto.
+      - unfold swap_down_right.
+        exists v0, ls0, rs0; tauto.
+    + eapply swap_down_right_hold; eauto.
+    + eapply MaxHeap_tree_down_hold_right; eauto.
+      - unfold get_list_val in H13; simpl in H13.
+        replace (2 * n) with (n * 2) in H13 by lia; lia.
+      - rewrite <- left_son_check_equal; eauto.
+  }
+Qed.
+
+(* Lemma Down_tree_list_succeed_clos_refl_trans: forall (l l': list_state) (t: tree_state),
+  list_on_tree_state l t -> (clos_refl_trans list_down_succeed) l l' -> MaxHeap_tree_up t ->
+  exists t', (clos_refl_trans tree_up_succeed) t t' /\ list_on_tree_state l' t' /\ MaxHeap_tree_up t'.
+Proof.
+Admitted. *)
+
+Lemma Down_tree_list_fail: forall (l: list_state) (t: tree_state),
+  list_on_tree_state l t -> list_down_fail l l ->
+  tree_down_fail t t.
+Proof.
+  intros.
+  unfold list_down_fail in H0.
+  destruct l as [l n].
+  destruct t as [pt tr].
+  unfold tree_down_fail.
+  revert H0; unfold_RELS_tac; intros; simpl.
+  unfold list_on_tree_state in H.
+  unfold list_on_tree_state_fix in H.
+  simpl in H.
+  destruct H.
+  destruct H0 as [[? ?] ?]; clear H3.
+  unfold left_son_check_list in H0.
+  unfold left_son in H0; simpl in H0.
+  apply not_and_or in H0.
+  unfold right_son_check_list in H2.
+  unfold right_son in H2; simpl in H2.
+  apply not_and_or in H2.
+  unfold legal_list_state in H0; simpl in H0.
+  unfold legal_list_state in H2; simpl in H2.
+  assert (n >= 1). {
+    inversion H; lia.
+  }
+  destruct H2.
+  + apply not_and_or in H2.
+    destruct H2; [ | lia].
+    destruct H0.
+    - apply not_and_or in H0.
+      destruct H0; [ | lia].
+      inversion H1.
+      * inversion H.
+        
+Admitted.
+
+Lemma Down_fail_impl_MaxHeap: forall (t: tree_state),
+  tree_down_fail t t -> MaxHeap_tree_down t -> MaxHeap (tree_compose (fst t) (snd t)).
+Proof.
+Admitted.
+
+Lemma Down_tree_list_rel: forall (l l': list_state) (t: tree_state),
+  list_on_tree_state l t -> heap_list_down l l' -> MaxHeap_tree_down t ->
+  exists t', heap_tree_down t t' /\ list_on_tree_state l' t' /\ MaxHeap (tree_compose (fst t') (snd t')).
+Proof.
+Admitted.
